Regex/Lemmas.lean
@@ -16,3 +16,9 @@ theorem String.eq_of_append_of_eq_of_append {s s₁ s₂ : String} (h : s = s₁
 theorem Nat.eq_of_ge_of_lt {m n : Nat} (ge : m ≥ n) (lt : m < n + 1) : m = n := by
   have le : m ≤ n := Nat.le_of_lt_succ lt
   exact Nat.le_antisymm le ge
+
+theorem Array.singleton_get (i : Fin 1) :
+  #[v][i] = v := by
+  match i with
+  | ⟨0, isLt⟩ => rfl
+  | ⟨i' + 1, _⟩ => contradiction
